VisualProof/Rule/Soundness/WirePrimitive/Content.lean
@@ -41,8 +41,10 @@ theorem Wrap.sound_iff {outer : List Sig} {source target : Region outer}
     ∀ (model : Model) (env : Values model outer),
       denoteRegion model env source ↔ denoteRegion model env target := by
   cases step with
-  | @mk arguments before after items itemsResult =>
+  | mk description =>
+    rcases description with ⟨arguments, before, after, items, itemsResult⟩
     intro model env
+    simp only [Wrap.Description.source, Wrap.Description.target]
     simp only [denoteRegion_mk]
     rw [Region.denote_adjoinAt]
     constructor
@@ -194,8 +196,10 @@ theorem Split.sound_iff {outer : List Sig} {source target : Region outer}
     ∀ (model : Model) (env : Values model outer),
       denoteRegion model env source ↔ denoteRegion model env target := by
   cases step with
-  | @mk arguments before after items itemsResult =>
+  | mk description =>
+    rcases description with ⟨arguments, before, after, items, itemsResult⟩
     intro model env
+    simp only [Split.Description.source, Split.Description.target]
     simp only [denoteRegion_mk]
     rw [Region.denote_adjoinAt]
     constructor
@@ -348,8 +352,10 @@ theorem Delete.sound {outer : List Sig} {applied empty : Region outer}
     ∀ (model : Model) (env : Values model outer),
       denoteRegion model env empty → denoteRegion model env applied := by
   cases step with
-  | @mk arguments before after items itemsResult =>
+  | mk description =>
+    rcases description with ⟨arguments, before, after, items, itemsResult⟩
     intro model env
+    simp only [Delete.Description.source, Delete.Description.target]
     simp only [denoteRegion_mk]
     rw [Region.denote_adjoinAt]
     rintro ⟨targetLocal, _, targetDenotes⟩
